abp/Medium/medsBelow.thy
@@ -1,25 +1,22 @@
 theory medsBelow
 
-imports medFairAut medUnfairAut
+imports abpGenerat.Fair99MediumAutomaton abpGenerat.FairMediumAutomaton
 
 begin
 
 
-lemma meds_transition_h_below: "medFairTransitionH s m \<subseteq> medUnfairTransitionH s m"
+lemma meds_transition_h_below: "(fairMediumTransitionH (s,m)) \<sqsubseteq> (fair99MediumTransitionH (s,m))"
   apply(cases m)
    apply(cases s)
-  by auto
-  
-lemma meds_aut_below: "medUnfairAut \<sqsubseteq> medFairAut"
+  sorry
+
+lemma meds_aut_below: "fairMediumAutomaton \<sqsubseteq> fair99MediumAutomaton"
   apply(rule nda_belowI)
      apply simp_all
-   apply(simp add: ndaInitialState.rep_eq medFairAut.rep_eq medUnfairAut.rep_eq)
-  apply(simp add: ndaTransition.rep_eq medFairAut.rep_eq medUnfairAut.rep_eq)
-  apply(auto simp add: below_fun_def less_set_def)
-  using meds_transition_h_below by fastforce
+   apply(simp add: fairMediumInitials_def fair99MediumInitials_def)
+  sorry
 
-lemma meds_below: "medUnfair s \<sqsubseteq> medFair s"
-  unfolding medUnfair_def medFair_def
-  by (simp add: fun_belowD meds_aut_below monofunE nda_h_mono)
+lemma meds_below: "fairMediumStep s \<sqsubseteq> fair99MediumStep s"
+  sorry
 
 end
